<?xml version="1.0"?>


<!DOCTYPE rdf:RDF [
    <!ENTITY dct "http://purl.org/dc/terms/" >
    <!ENTITY cito "http://purl.org/spar/cito/" >
    <!ENTITY owl "http://www.w3.org/2002/07/owl#" >
    <!ENTITY dc "http://purl.org/dc/elements/1.1/" >
    <!ENTITY xsd "http://www.w3.org/2001/XMLSchema#" >
    <!ENTITY skos "http://www.w3.org/2004/02/skos/core#" >
    <!ENTITY rdfs "http://www.w3.org/2000/01/rdf-schema#" >
    <!ENTITY rdf "http://www.w3.org/1999/02/22-rdf-syntax-ns#" >
    <!ENTITY bino "http://www.davidstuart.co.uk/ontologies/bino#" >
]>


<rdf:RDF xmlns="http://www.w3.org/2002/07/owl#"
     xml:base="http://www.w3.org/2002/07/owl"
     xmlns:dc="http://purl.org/dc/elements/1.1/"
     xmlns:rdfs="http://www.w3.org/2000/01/rdf-schema#"
     xmlns:cito="http://purl.org/spar/cito/"
     xmlns:dct="http://purl.org/dc/terms/"
     xmlns:owl="http://www.w3.org/2002/07/owl#"
     xmlns:xsd="http://www.w3.org/2001/XMLSchema#"
     xmlns:rdf="http://www.w3.org/1999/02/22-rdf-syntax-ns#"
     xmlns:skos="http://www.w3.org/2004/02/skos/core#"
     xmlns:bino="http://www.davidstuart.co.uk/ontologies/bino#">
    <Ontology rdf:about="http://www.davidstuart.co.uk/ontologies/bino">
        <imports rdf:resource="http://purl.org/dc/terms/"/>
        <imports rdf:resource="http://purl.org/spar/cito/"/>
        <imports rdf:resource="http://www.w3.org/2004/02/skos/core#"/>
    </Ontology>
    


    <!-- 
    ///////////////////////////////////////////////////////////////////////////////////////
    //
    // Object Properties
    //
    ///////////////////////////////////////////////////////////////////////////////////////
     -->

    


    <!-- http://purl.org/dc/terms/type -->

    <ObjectProperty rdf:about="&dct;type"/>
    


    <!-- http://purl.org/spar/cito/cites -->

    <ObjectProperty rdf:about="&cito;cites"/>
    


    <!-- http://purl.org/spar/cito/describes -->

    <ObjectProperty rdf:about="&cito;describes"/>
    


    <!-- http://purl.org/spar/cito/discusses -->

    <ObjectProperty rdf:about="&cito;discusses"/>
    


    <!-- http://purl.org/spar/cito/extends -->

    <ObjectProperty rdf:about="&cito;extends"/>
    


    <!-- http://purl.org/spar/cito/usesMethodIn -->

    <ObjectProperty rdf:about="&cito;usesMethodIn"/>
    


    <!-- http://www.davidstuart.co.uk/ontologies/bino#hasConstraint -->

    <ObjectProperty rdf:about="&bino;hasConstraint">
        <rdfs:label xml:lang="en">has constraint</rdfs:label>
        <rdfs:comment xml:lang="en">Associates an Indicator (the subject of the triple) with a limitation that is placed on an Indicator.

For example, the Journal Impact Factor hasConstraint time, as only citations from a two-year period are counted. 
</rdfs:comment>
    </ObjectProperty>
    


    <!-- http://www.davidstuart.co.uk/ontologies/bino#hasVariable -->

    <ObjectProperty rdf:about="&bino;hasVariable">
        <rdfs:label xml:lang="en">has variable</rdfs:label>
        <rdfs:comment xml:lang="en">Associates an Indicator (the subject of the triple) with an input that is used in the calculation of that indicator and is expected to vary for different objects of analysis.</rdfs:comment>
    </ObjectProperty>
    


    <!-- http://www.davidstuart.co.uk/ontologies/bino#objectOfAnalysis -->

    <ObjectProperty rdf:about="&bino;objectOfAnalysis">
        <rdfs:label xml:lang="en">object of analysis</rdfs:label>
        <rdfs:comment xml:lang="en">Associates an Indicator (the subject of the triple) with a term that reflects the type of object that is the focus of the analysis. 

Typical examples include units of publication (e.g., article, journal, publisher) or units of authorship/research (e.g., researcher, research group, department, university, country).
</rdfs:comment>
    </ObjectProperty>
    


    <!-- 
    ///////////////////////////////////////////////////////////////////////////////////////
    //
    // Data properties
    //
    ///////////////////////////////////////////////////////////////////////////////////////
     -->

    


    <!-- http://purl.org/dc/terms/bibliographicCitation -->

    <DatatypeProperty rdf:about="&dct;bibliographicCitation"/>
    


    <!-- http://purl.org/dc/terms/creator -->

    <DatatypeProperty rdf:about="&dct;creator"/>
    


    <!-- http://purl.org/dc/terms/issued -->

    <DatatypeProperty rdf:about="&dct;issued"/>
    


    <!-- http://purl.org/dc/terms/publisher -->

    <DatatypeProperty rdf:about="&dct;publisher"/>
    


    <!-- http://purl.org/dc/terms/title -->

    <DatatypeProperty rdf:about="&dct;title"/>
    


    <!-- http://www.w3.org/2004/02/skos/core#altLabel -->

    <DatatypeProperty rdf:about="&skos;altLabel"/>
    


    <!-- http://www.w3.org/2004/02/skos/core#broader -->

    <DatatypeProperty rdf:about="&skos;broader"/>
    


    <!-- http://www.w3.org/2004/02/skos/core#narrower -->

    <DatatypeProperty rdf:about="&skos;narrower"/>
    


    <!-- http://www.w3.org/2004/02/skos/core#note -->

    <DatatypeProperty rdf:about="&skos;note"/>
    


    <!-- http://www.w3.org/2004/02/skos/core#prefLabel -->

    <DatatypeProperty rdf:about="&skos;prefLabel"/>
    


    <!-- http://www.w3.org/2004/02/skos/core#related -->

    <DatatypeProperty rdf:about="&skos;related"/>
    


    <!-- 
    ///////////////////////////////////////////////////////////////////////////////////////
    //
    // Classes
    //
    ///////////////////////////////////////////////////////////////////////////////////////
     -->

    


    <!-- http://purl.org/dc/terms/BibliographicResource -->

    <Class rdf:about="&dct;BibliographicResource"/>
    


    <!-- http://www.davidstuart.co.uk/ontologies/bino#Indicator -->

    <Class rdf:about="&bino;Indicator">
        <rdfs:label xml:lang="en">Indicator</rdfs:label>
        <rdfs:comment xml:lang="en">A bibliometric indicator; a statistical method applied to a particular aspect of communication. 

&apos;Bibliometric&apos; is not limited solely to traditional forms of academic publication (e.g., journal articles), but includes altmetric and webometric indicators.</rdfs:comment>
    </Class>
    


    <!-- http://www.w3.org/2004/02/skos/core#Concept -->

    <Class rdf:about="&skos;Concept"/>
</rdf:RDF>



<!-- Generated by the OWL API (version 3.4.2) http://owlapi.sourceforge.net -->

